Tactic improvements.

rocq-osiris/examples/proofs/fold_array.v
@@ -12,10 +12,35 @@ Section verification.
 
   Open Scope Z.
 
+  (* Some helpful lemmas about sums. *)
+
+  Definition gauss_summation n := n * (n + 1) / 2.
+
+  Lemma gauss_summation_0 :
+    gauss_summation 0 = 0.
+  Proof.
+    unfold gauss_summation.
+    rewrite Z.mul_0_l Zdiv_0_l.
+    reflexivity.
+  Qed.
+
+  Lemma gauss_summation_incr n :
+    gauss_summation n + (n + 1) = gauss_summation (n + 1).
+  Proof.
+    unfold gauss_summation.
+    replace (n + 1 + 1) with (n + 2) by lia.
+    replace ((n + 1) * (n + 2)) with ((n + 1) * n + (n + 1) * 2) by lia.
+    rewrite Z.div_add; last lia. rewrite Z.mul_comm. reflexivity.
+  Qed.
+
+  (* The specification of our function:
+     the precondition is [0 ≤ n ≤ max_array]
+     the postcondition is [λ i, ⌜i = gaus_summation n⌝]. *)
+
   Definition sum_spec : Z → microvx → iProp Σ :=
     λ n m,
       (⌜0 ≤ n ≤ max_array⌝ -∗
-       imp m {{ λ i, ⌜i = n * (n + 1) / 2⌝ }})%I.
+       imp m {{ λ i, ⌜i = gauss_summation n⌝ }})%I.
 
   Definition esum := EAnonFun __fun2.
 
@@ -28,50 +53,55 @@ Section verification.
     iApply imp_EAnon_pers.
     iIntros "!>" (n Hpos).
     iApply imp_please; iNext.
+
     (* let a = .. *)
     iApply (imp_ELet_var (B:=array)).
-    { (* Array.init n (fun i -> i +) *)
+    { (* Start by initializing an array with
+         [Array.init n (fun i -> i +)] *)
       imp_app τ[Z;val].
       (* (fun i -> i + 1) *)
       { iApply (imp_EAnon_pers τ[Z] (λ i m, imp m {{ λ j, ⌜(j = i + 1)%Z⌝ }})%I).
         iIntros (i) "!>". iApply imp_please; iNext.
-        iApply imp_EIntAdd. imp_path. iApply imp_EInt.
-        iIntros "!>" (? j) "-> ->". auto. }
+        imp_arith. iIntros "!>" (? j) "-> ->". auto. }
       iIntros (f ?) "-> #Hf %m Hm".
+      (* We weaken the spec of [Array.init] to one where the function
+         does not depend on the previously initialized elements. *)
       iPoseProof (weaken_init_spec with "Hm") as "Hm".
-      iApply ("Hm" $! Z _ _ _ Hpos).
+      iApply ("Hm" $! Z with "[//]").
       iIntros "!> !>".
       iApply (iSpec_mono with "Hf").
       iIntros (i m') "$ Hbound //". }
-    iIntros (a) "(%xs & %Hlenxs & HownArr & #Hxs)".
-    (* Array.fold_left (+) 0 a *)
+
+    (* Prove rhs of [let a] *)
+    iIntros (a) "(%xs & <- & HownArr & #Hxs)".
+    (* We now prove the fold which returns the final result:
+       [Array.fold_left (+) 0 a]. *)
     imp_app τ[val;Z;array].
     iIntros (??) "-> %add #Hadd_ -> %m Hm".
 
-    iSpecialize ("Hm" $! Z _ _ _ xs (λ acc elems, let n := length elems in ⌜acc = n * (n + 1) / 2⌝)%I).
     iPoseProof (slice_of_own with "HownArr") as "(#Harr & Hslice)"; first reflexivity.
-    iSpecialize ("Hm" with "Harr Hslice").
-    iApply (imp_mono_ret with "[-]").
+    iSpecialize ("Hm"
+                   $! Z _ _ _ _ (λ acc elems, ⌜acc = gauss_summation (length elems)⌝)%I
+                  with "Harr Hslice").
+    (* Show that we can drop the ownership of the array *)
+    iApply (imp_mono_ret (λ v, ⌜v = _⌝ ∗ _)%I with "[-]");
+      last (iIntros "!>" (?) "(-> & _)"; iPureIntro; reflexivity).
 
-    - iApply "Hm".
-      + iIntros "!>".
-        iApply (iSpec_mono with "Hadd_").
-        iIntros (i j m') "Hm' %visited %Hprefix %Hacc".
-        iApply (imp_mono_ret with "Hm'").
-        iIntros (? ->). length.
-        destruct Hprefix as (ys & ->).
-        iPoseProof (big_sepLZ_lookup_acc _ _ (length visited) j with "Hxs")
-          as "(%Hvisited & _)"; first by lookup.
-        iPureIntro.
-        (* Painful arithmetic rewriting. *)
-        remember (length visited) as v.
-        replace (v + 1 + 1) with (v + 2) by lia.
-        rewrite -Hvisited in Hacc |-*; rewrite Hacc.
-        replace (j * (v + 2)) with (j * v + j * 2) by lia.
-        rewrite Z.div_add; last lia. rewrite Z.mul_comm. reflexivity.
-      + iPureIntro. length. rewrite Z.mul_0_l Zdiv_0_l. reflexivity.
-    - iIntros "!>" (acc) "(%Hacc & Hslice)".
-      iPureIntro. rewrite Hacc Hlenxs. reflexivity.
+    iApply "Hm".
+    + (* Subgoal: show that adding each successive element preserves the invariant. *)
+      iIntros "!>".
+      iApply (iSpec_mono with "Hadd_").
+      iIntros (i j m') "Hm' %visited %Hprefix ->".
+      iApply (imp_mono_ret with "Hm'").
+      iIntros (? ->). length.
+      destruct Hprefix as (ys & ->).
+      iPoseProof (big_sepLZ_lookup_acc _ _ (length visited) j with "Hxs")
+        as "(-> & _)"; first by lookup.
+      iPureIntro.
+      apply gauss_summation_incr.
+
+    + (* Show that the invariant holds initially. *)
+      iPureIntro. length. by rewrite gauss_summation_0.
   Qed.
 
   Lemma module_proof η :
